ckp

formal/task01/list_spec.v
@@ -2,12 +2,142 @@
 
 Require Import VST.floyd.proofauto.
 Require Import VST.floyd.library.
-Require Import  hash.
+Require Import Task1.state_list.
+
 Instance CompSpecs : compspecs. make_compspecs prog. Defined.
 Definition Vprog : varspecs.  mk_varspecs prog. Defined.
 
-Require Import VST.msl.wand_frame.
-Require Import VST.msl.iter_sepcon.
-Require Import VST.floyd.reassoc_seq.
-Require Import VST.floyd.field_at_wand.
-Require Import Hashfun.
+(*
+  We define versions of the specs that take the identifiers and type arguments so that
+  We can be imported into different separate compilation units. 
+
+Definition strchr_spec' {CSX: compspecs} (_strchr _str _c: positive) :=
+ DECLARE _strchr
+  WITH sh: share, str : val, s : list byte, c : byte
+  PRE  [ _str OF tptr tschar, _c OF tint ]
+    PROP (readable_share sh; c <> Byte.zero)
+    LOCAL (temp _str str; temp _c (Vbyte c))
+    SEP (cstring sh s str)
+  POST [ tptr tschar ]
+   EX r : val,
+    PROP ((exists i, Znth i s = c /\ Forall (fun d => d<>c) (sublist 0 i s)
+                     /\ r = offset_val i str)
+       \/ (Forall (fun d => d<>c) s /\ r = nullval))
+    LOCAL (temp ret_temp r)
+    SEP (cstring sh s str).
+
+ *)
+
+(* type of the list cell *)
+Definition tcell := Tstruct _s_state_list noattr.
+
+(* Field ident holding the data. *)
+Definition data_id := _data.
+
+(* Field ident holding the pointer to next cell *)
+Definition next_id := _next.
+
+(* Type of the data *)
+Definition tdata := Tstruct _s_state noattr.
+
+(* Coq type representing tdata *)
+Definition rdata := Eval compute in reptype tdata.
+
+(* Coq type representing tcell *)
+Definition rcell := Eval compute in reptype tcell.
+
+(* Define what it means for a pointer to hold a list cell *)
+Definition list_cell (data: rdata) (next: val) (p: val): mpred :=
+ data_at Ews tcell (data, next) p * malloc_token Ews tcell p.
+
+Definition list_cell_local_facts:
+  forall data next p, list_cell data next p |-- !! isptr p.
+Proof. intros. unfold list_cell. entailer!. Qed.
+Hint Resolve list_cell_local_facts: saturate_local.
+
+Definition list_cell_valid_pointer:
+  forall data next p, list_cell data next p |-- valid_pointer p.
+Proof. intros. unfold list_cell. entailer!. Qed.
+Hint Resolve list_cell_valid_pointer: valid_pointer.
+
+Lemma listcell_fold: forall data p' p,
+    data_at Ews tcell (data, p') p
+    * malloc_token Ews tcell p
+                   |-- list_cell data p' p.
+Proof.
+  intros.
+  unfold list_cell.
+  entailer!.
+Qed.
+
+Fixpoint listrep (sigma: list rdata) (x: val) : mpred :=
+ match sigma with
+ | d::hs => EX y: val, list_cell d y x * listrep hs y
+ | nil => !! (x = nullval) && emp
+ end.
+
+Lemma listrep_local_prop: forall sigma p, listrep sigma p |--
+        !! (is_pointer_or_null p  /\ (p=nullval <-> sigma=nil)).
+Proof.
+  intro sigma.
+  induction sigma as [| d tl].
+  { (* sigma is nil *)
+    simpl.
+    entailer!.
+    split; reflexivity.
+  }
+  { (* sigma is d :: tl *)
+    intro p'.
+    simpl.
+    entailer.
+    saturate_local.
+    entailer!.
+    split.
+    {
+      intro.
+      subst p'.
+      contradiction.
+    }
+    {
+      intro.
+      inversion H0.
+    }
+  }
+Qed.
+
+Hint Resolve listrep_local_prop : saturate_local.
+
+Lemma listrep_valid_pointer:
+  forall sigma p, listrep sigma p |-- valid_pointer p.
+Proof.
+  intro sigma.
+  induction sigma as [| d tl].
+  { (* sigma is nil *)
+    simpl.
+    entailer!.
+  }
+  { (* sigma is d :: tl *)
+    intro p'.
+    simpl.
+    entailer.
+  }
+Qed.
+
+Hint Resolve listrep_valid_pointer : valid_pointer.
+
+Definition new_cell_id := _new_state_list.
+Definition new_cell_spec : ident * funspec :=
+ DECLARE new_cell_id
+ WITH sh: share, data: rdata, next: val, gv: globals
+ PRE [ data_id OF rdata, next_id OF tptr tcell ]
+   PROP(readable_share sh)
+   LOCAL(temp data_id data; temp next_id next; gvars gv)
+   SEP(mem_mgr gv)
+ POST [ tptr tcell ]
+   EX p:val, PROP()
+      LOCAL(temp ret_temp p)
+      SEP(list_cell data next p; mem_mgr gv).
+
+
+
+
